useram_key_uncompromised_setup theorem

src/AttarchProperties.v
@@ -40,7 +40,7 @@ Proof.
       tentails! in *.
       intros .
       destruct H5 as (acc & a & lookup & Hacc & ->).
-      destruct a as [? a]; change ⟨_, a⟩ with (box a) in *.
+      unbox a.
       simpl_rws.
       follows eapply IHHstar.
     + invc H; invc H0; rw_solver.
@@ -48,38 +48,60 @@ Qed.
 
 
 Definition useram_key_secure : tprop attarch_state := <[λ '(_, Γ),
-  forall c key_t (key: key_t),
-    read Γ c "useram_key" key -> 
+  forall c,
+    read Γ c "useram_key" good_useram_key -> 
     c = "useram"
 ]>.
 
-(* Definition finish_setup : tprop attarch_state := <[λ '(l, _),
-  exists l', l = sel4_run l' (vm_run useram_listen)
+(* Definition useram_key_released : tprop attarch_state := <[λ '(l, _),
+  exists vl, l = sel4_run platam_listen vl
 ]>. *)
 
-Definition setup_finished : tprop attarch_state := <[λ '(l, _),
-  exists pl ul, 
-    l = sel4_run pl (vm_run ul) /\
+Definition useram_key_released : tprop attarch_state := <[λ '(l, _),
+  exists pl ul,
+    l = sel4_run pl (vm_run ul) /\ 
     ul <> useram_wait_key
 ]>.
 
 Theorem useram_key_uncompromised_setup : forall s0,
   is_init_attarch_state s0 ->
-  attarch_trans @s0 ⊨ A[useram_key_secure W setup_finished].
+  attarch_trans @s0 ⊨ A[useram_key_secure W useram_key_released].
 Proof.
   intros s0 s0_init.
+  apply AW_weaken_left
+    with (P := <[λ '(_, Γ), forall acc v,
+      Γ "useram_key" = Some (acc, box v) ->
+      v <> good_useram_key
+    ]>).
+  { intros [l Γ].
+    tintro H.
+    tentails! in *.
+    intros.
+    exfalso.
+    destruct H0 as (? & ? & ?).
+    follows eapply H. }
   apply AW_intro_weak.
   - left.
-    destruct or s0_init; rewritec s0_init;
-    follows tentails!.
-  - intros * Hstar [Hsecure Hnot_finished] * H.
-    invc H; try (left; rw_solver).
-    + left. invc H; rw_solver. 
+    destruct or s0_init; 
+    rewrite s0_init;
+    rw_solver.
+  - intros * Hstar Hs' * H.
+    destruct Hs' as [Hs'l Hs'r].
+    invc H.
+    + left. rw_solver with find inject.
+    + left. rw_solver with find inject.
+    + invc H; left; rw_solver.
     + invc H; invc H0; try (left + right; rw_solver).
-      (* not true at the moment. Need platam to inspect useram
-         before releasing key!
-       *)
-Abort.
+      left.
+      tentails! in *.
+      destruct H as (acc & V & v & lookup & ->).
+      intros acc' key Hacc'.
+      inject Hacc'.
+      eapply Hs'l.
+      eassumption.
+    + left. rw_solver.
+Qed.
+ 
 
 Close Scope tprop_scope.
 Close Scope string_scope.
